atomic_sync.v
@@ -1,0 +1,103 @@
+From iris.program_logic Require Export weakestpre hoare.
+From iris.heap_lang Require Export lang.
+From iris.heap_lang Require Import proofmode notation.
+From iris.heap_lang.lib Require Import spin_lock.
+From iris.tests Require Import atomic misc.
+From iris.algebra Require Import dec_agree frac.
+From iris.program_logic Require Import auth.
+
+Definition syncR := prodR fracR (dec_agreeR val).
+Class syncG Σ := sync_tokG :> inG Σ syncR.
+Definition syncΣ : gFunctors := #[GFunctor (constRF syncR)].
+
+Instance subG_syncΣ {Σ} : subG syncΣ Σ → syncG Σ.
+Proof. by intros ?%subG_inG. Qed.
+
+Section atomic_sync.
+  Context `{!heapG Σ, !lockG Σ, !inG Σ (prodR fracR (dec_agreeR val))} (N : namespace).
+
+  Definition A := val. (* FIXME: can't use a general A instead of val *)
+
+  Definition gHalf (γ: gname) g : iProp Σ := own γ ((1/2)%Qp, DecAgree g).
+
+  Definition atomic_triple'
+             (α: val → iProp Σ)
+             (β: val → A → A → val → iProp Σ)
+             (Ei Eo: coPset)
+             (f x: val) γ : iProp Σ :=
+    (∀ P Q, (∀ g, (P x ={Eo, Ei}=> gHalf γ g ★ □ α x) ★
+                  (gHalf γ g ★ □ α x ={Ei, Eo}=> P x) ★
+                  (∀ g' r, gHalf γ g' ★ β x g g' r ={Ei, Eo}=> Q x r))
+            -★ {{ P x }} f x {{ v, Q x v }})%I.
+
+  Definition sync (syncer: val) : val :=
+    λ: "f_cons" "f_seq",
+        let: "l"  := "f_cons" #() in
+        syncer ("f_seq" "l").
+
+  Definition seq_spec (f: val) (ϕ: val → A → iProp Σ) α β (E: coPset) :=
+      ∀ (Φ: val → iProp Σ) (l: val),
+         {{ True }} f l {{ f', ■ (∀ (x: val) (Φ: val → iProp Σ) (g: A),
+                               heapN ⊥ N →
+                               heap_ctx ★ ϕ l g ★ □ α x ★
+                               (∀ (v: val) (g': A), ϕ l g' -★ β x g g' v -★ |={E}=> Φ v)
+                               ⊢ WP f' x @ E {{ Φ }} )}}.
+
+  Definition cons_spec (f: val) (g: A) ϕ :=
+      ∀ Φ: val → iProp Σ, heapN ⊥ N →
+        heap_ctx ★ (∀ (l: val) (γ: gname), ϕ l g -★ gHalf γ g -★ gHalf γ g -★ Φ l)
+        ⊢ WP f #() {{ Φ }}.
+
+  Definition synced R (f' f: val) :=
+    (∀ P Q (x: val), ({{ R ★ P x }} f x {{ v, R ★ Q x v }}) → ({{ P x }} f' x {{ v, Q x v }}))%I.
+
+  Definition mk_sync_spec (syncer: val) :=
+    ∀ f R (Φ: val → iProp Σ),
+      heapN ⊥ N → 
+      heap_ctx ★ R ★ (∀ f', □ synced R f' f -★ Φ f') ⊢ WP syncer f {{ Φ }}.
+  
+  Lemma atomic_spec (syncer f_cons f_seq: val) (ϕ: val → A → iProp Σ) α β Ei:
+      ∀ (g0: A),
+        heapN ⊥ N → seq_spec f_seq ϕ α β ⊤ → cons_spec f_cons g0 ϕ →
+        mk_sync_spec syncer →
+        heap_ctx
+        ⊢ WP (sync syncer) f_cons f_seq {{ f, ∃ γ, gHalf γ g0 ★ ∀ x, □ atomic_triple' α β Ei ⊤ f x γ  }}.
+  Proof.
+    iIntros (g0 HN Hseq Hcons Hsync) "#Hh". repeat wp_let.
+    wp_bind (f_cons _). iApply Hcons=>//. iFrame "Hh".
+    iIntros (l γ) "Hϕ HFull HFrag".
+    wp_let. wp_bind (f_seq _)%E.
+    iApply wp_wand_r. iSplitR; first by iApply (Hseq with "[]")=>//.
+    iIntros (f Hf). iApply (Hsync f (∃ g: A, ϕ l g ★ gHalf γ g)%I)=>//.
+    iFrame "#". iSplitL "HFull Hϕ".
+    { iExists g0. by iFrame. }
+    iIntros (f') "#Hflatten".
+    iExists γ. iFrame.
+    iIntros (x). iAlways.
+    rewrite /atomic_triple'.
+    iIntros (P Q) "#Hvss".
+    rewrite /synced.
+    iSpecialize ("Hflatten" $! P Q).
+    iApply ("Hflatten" with "[]").
+    iAlways. iIntros "[HR HP]". iDestruct "HR" as (g) "[Hϕ HgFull]".
+    (* we should view shift at this point *)
+    iDestruct ("Hvss" $! g) as "[Hvs1 [Hvs2 Hvs3]]".
+    iApply pvs_wp.
+    iVs ("Hvs1" with "HP") as "[HgFrag #Hα]".
+    iVs ("Hvs2" with "[HgFrag]") as "HP"; first by iFrame.
+    iVsIntro. iApply Hf=>//.
+    iFrame "Hh Hϕ". iSplitR; first done. iIntros (ret g') "Hϕ' Hβ".
+    iVs ("Hvs1" with "HP") as "[HgFrag _]".
+    iCombine "HgFull" "HgFrag" as "Hg".
+    rewrite /gHalf.
+    iAssert (|=r=> own γ (((1 / 2)%Qp, DecAgree g') ⋅ ((1 / 2)%Qp, DecAgree g')))%I with "[Hg]" as "Hupd".
+    { iApply (own_update); last by iAssumption. apply pair_l_frac_update. }
+    iVs "Hupd" as "[HgFull HgFrag]".
+    iVs ("Hvs3" $! g' ret with "[HgFrag Hβ]"); first by iFrame.
+    iVsIntro.
+    iSplitL "HgFull Hϕ'".
+    - iExists g'. by iFrame.
+    - done.
+  Qed.
+  
+End atomic_sync.
